### lookahead

$$(?=(?=(aa|b)^*b)(bb|a)^+a)a(a|b)^*a \approx (aa)^+(bb)^+a((a|b)^*a)?$$

Let's look at it broken down into parts:
$$(?= (aa|b)^*b)(bb|a)^+a$$

Because the first part $(aa|b)^*b.^*$ (e.g., $(aa)^*b$) and the second part $(aa)^*(bb)^+a.^*$

In the last step, from $(aa)^*(bb)^+a.^*$ and $a(a|b)^*a$, we get '$a$' from
$(bb|\underline{a})^+a \leftrightarrow \underline{a}(a|b)^*a \leftrightarrow \underline{a}(bb|a)^*a$

And after simplifications ($(aa|b)^*b.^* \to (aa)^+ \dots$), we get $$(aa)^+(bb)^+a((a|b)^*a)?$$
### lookbehind

$$(ab)^*b(ba)^*a(?<=(baa|bb)^+(a|b)^*) \approx (ab)^*b(ba)^+a$$
$$.^*(baa|bb)^+.^* \to .^*(baa|bb) .^*$$
$$(ab)^+b(ba)^*a|\cancel{(ab)^*}b(ba)^*$$

Because having looked at it $(ab)^*b$ as 1, $(ba)^*a$ as 2:
- 1 not empty $\Rightarrow$ 2 not empty?
- 1 empty $\Rightarrow$ 2 not empty
$$(ab)^*b(ba)^*a(?<=(baa|bb)^+(aa|b)^*)$$
$$.^*(baa|bb)(aa|b)^*$$
Start: $(baa|bb)^*$
Middle: $.^*(baa|bb)(aa|b)^*$
End: $(ab)^*bbaa$

And after simplifications, we get $$(ab)^*b(ba)^+a$$
